

Vector Differential Calculus

Definitions

① Scalar point function:

If to each point $P(R)$ of a region E in space there corresponds to a definite scalar denoted by $f(R)$, then $f(R)$ is called a scalar point function in E . The region E is called a scalar field.

② Vector point function:

If to each point $P(R)$ of a region E in space there corresponds a definite vector denoted by $F(R)$ then it is called the vector point function in E . The region E is called a vector field.

③ Vector operator ∇

∇ (read as del) is defined as $\nabla = \hat{i} \frac{\partial}{\partial x} + \hat{j} \frac{\partial}{\partial y} + \hat{k} \frac{\partial}{\partial z}$

④ Gradient of f

the vector function ∇f is defined as the gradient of the scalar point function f and is del written as $\text{grad } f$.

$$\text{grad } f = \nabla f = \bar{i} \frac{\partial f}{\partial x} + \bar{j} \frac{\partial f}{\partial y} + \bar{k} \frac{\partial f}{\partial z}$$

⑤ Directional derivative:

For a scalar point function f , and a unit vector \bar{u} , the directional derivative is given by the dot product of ∇f and the unit vector \bar{u} at the point

(x_0, y_0, z_0) .

$$\text{Directional derivative at the point } (x_0, y_0, z_0) = \bar{u} \cdot \nabla f(x_0, y_0, z_0)$$

⑥ Divergence:

The divergence of a continuously differentiable vector point function F is denoted by $\text{div } F$ and is defined by

the equation

$$\text{div } F = \nabla \cdot F = \bar{i} \frac{\partial F}{\partial x} + \bar{j} \frac{\partial F}{\partial y} + \bar{k} \frac{\partial F}{\partial z}$$

$$\text{If } F = f_1 \bar{i} + f_2 \bar{j} + f_3 \bar{k}$$

$$\begin{aligned} \text{div } F = \nabla \cdot F &= \left(\bar{i} \frac{\partial}{\partial x} + \bar{j} \frac{\partial}{\partial y} + \bar{k} \frac{\partial}{\partial z} \right) \cdot (f_1 \bar{i} + f_2 \bar{j} + f_3 \bar{k}) \\ &= \frac{\partial f_1}{\partial x} + \frac{\partial f_2}{\partial y} + \frac{\partial f_3}{\partial z} \end{aligned}$$

⑦ Curl : The curl of a continuously differentiable vector point function F is defined by the equation

$$\text{curl } F = \nabla \times F = \bar{i} \times \frac{\partial F}{\partial x} + \bar{j} \times \frac{\partial F}{\partial y} + \bar{k} \times \frac{\partial F}{\partial z}$$

If $F = f_1 \bar{i} + f_2 \bar{j} + f_3 \bar{k}$, then $\text{curl } F = \nabla \times F$

$$= \left(\bar{i} \frac{\partial}{\partial x} + \bar{j} \frac{\partial}{\partial y} + \bar{k} \frac{\partial}{\partial z} \right) \times (f_1 \bar{i} + f_2 \bar{j} + f_3 \bar{k})$$

$$= \begin{vmatrix} \bar{i} & \bar{j} & \bar{k} \\ \frac{\partial}{\partial x} & \frac{\partial}{\partial y} & \frac{\partial}{\partial z} \\ f_1 & f_2 & f_3 \end{vmatrix}$$

⑧ Solenoidal Vector:

If $\text{div } F = 0$ everywhere, then such a vector is called a solenoidal vector function

⑨ Irrotational Vector:

If the curl of the vector is zero then it is said to be irrotational, otherwise rotational.

Laplace Transforms

Definitions and solutions for Homework problems

Laplace Transforms:

Let $f(t)$ be a function of t defined for all positive values of t . Then the Laplace transforms of $f(t)$, denoted by $L\{f(t)\}$ is defined by

$$L\{f(t)\} = \int_0^{\infty} e^{-st} f(t) dt$$

provided that the integral exists. s is a parameter which may be a real or complex number.

Inverse Laplace Transforms

$L\{f(t)\}$ being clearly a function of s is briefly written as $\bar{f}(s)$ i.e., $L\{f(t)\} = \bar{f}(s)$, which can be written as $f(t) = L^{-1}\{\bar{f}(s)\}$

Transforms of elementary functions

① $L\{1\} = \frac{1}{s}$

$s > 0$

$$\int_0^{\infty} e^{-st} \cdot 1 dt = \left[\frac{e^{-st}}{-s} \right]_0^{\infty} = 0 + \frac{1}{s} = \frac{1}{s}$$

$$\textcircled{2} L(t^n) = \int_0^{\infty} t^n e^{-st} dt = \text{put } st = p$$

$$t = \frac{p}{s} \Rightarrow t^n = \left(\frac{p}{s}\right)^n$$

$$dt = \frac{dp}{s}$$

$$= \int_0^{\infty} \frac{p^n}{s^n} e^{-p} \frac{dp}{s} = \frac{1}{s^{n+1}} \int_0^{\infty} p^n e^{-p} dp$$

$$= \frac{\Gamma(n+1)}{s^{n+1}} = \frac{n!}{s^{n+1}} \quad \text{if } n > -1, \text{ and } s > 0.$$

$$\left(\int_0^{\infty} p^n e^{-p} dp = \Gamma(n+1) = n! \right)$$

$$\Gamma_{\frac{1}{2}} = \sqrt{\pi}$$

$$\textcircled{3} L(e^{at}) = \int_0^{\infty} e^{at} e^{-st} dt = \int_0^{\infty} e^{a-(s-a)t} dt$$

$$= \frac{e^{-(s-a)t}}{-(s-a)} \Big|_0^{\infty} = 0 + \frac{1}{(s-a)} = \frac{1}{s-a}$$

$$\textcircled{4} L(\sin at) = \int_0^{\infty} e^{-st} \sin at dt$$

1st Method: By integration by parts

$$\int_0^{\infty} e^{-st} \sin at dt = \sin at \frac{e^{-st}}{-s} - \int_0^{\infty} a \cos at \frac{e^{-st}}{-s} dt$$

$$= -\frac{s \sin at}{s} e^{-st} + \frac{a}{s} \int \cos at e^{-st} dt$$

$$= -\frac{s \sin at}{s} e^{-st} + \frac{a}{s} \left[\cos at \frac{e^{-st}}{-s} + \int s \sin at \frac{e^{-st}}{-s} dt \right]$$

$$= -\frac{s \sin at}{s} e^{-st} + \frac{a}{s} \left[-\frac{\cos at e^{-st}}{s} - \frac{a}{s} \int \sin at e^{-st} dt \right]$$

$$\text{let } \int e^{-st} \sin at dt = I$$

$$\Rightarrow I = -\frac{s \sin at}{s} e^{-st} - \frac{a}{s^2} \cos at e^{-st} - \frac{a^2}{s^2} I$$

$$\Rightarrow I + \frac{a^2}{s^2} I = -\frac{s \sin at}{s} e^{-st} - \frac{a}{s^2} \cos at e^{-st}$$

$$I = -\left(\frac{s^2}{s^2 + a^2} \right) \left(\frac{s \sin at}{s} e^{-st} + \frac{a}{s^2} \cos at e^{-st} \right)$$

$$= -\frac{1}{s^2 + a^2} \left(s \sin at e^{-st} + a \cos at e^{-st} \right)$$

$$I = -\frac{e^{-st}}{s^2 + a^2} (s \sin at + a \cos at)$$

$$\int_0^{\infty} e^{-st} \sin at dt = \left. -\frac{e^{-st}}{s^2 + a^2} (s \sin at + a \cos at) \right|_0^{\infty}$$

$$= \frac{1}{s^2 + a^2} (s \sin 0 + a \cos 0) = \underline{\underline{\frac{a}{s^2 + a^2}}}$$

$$L(a \sin at) = \frac{a}{s^2 + a^2} //$$

2nd Method: $e^{iat} = \cos at + i \sin at$
 $e^{-iat} = \cos at - i \sin at$

$$\frac{e^{ait} + e^{-ait}}{2} = \cos at$$

$$\frac{e^{ait} - e^{-ait}}{2i} = \sin at$$

$$L(\sin at) = \frac{h(e^{ait} - e^{-ait})}{2i}$$

$$= \frac{h(e^{ait}) - h(e^{-ait})}{2i} = \frac{\frac{1}{s-ai} - \frac{1}{s+ai}}{2i}$$

$$= \frac{s+ai - (s-ai)}{\frac{s^2 - (ai)^2}{2i}} = \frac{s+ai - s+ai}{(s^2 + a^2) 2i}$$

$$= \underline{\underline{\frac{a}{s^2 + a^2}}}$$

⑤ $L(\cos at) =$ Method 1: similar to ④

Method 2: $L(\cos at) = \frac{h(e^{ait} + e^{-ait})}{2}$
 $= \frac{h(e^{ait}) + h(e^{-ait})}{2}$
 $= \frac{\frac{1}{s-ai} + \frac{1}{s+ai}}{2}$

$$= \frac{(s+ai) + (s-ai)}{(s^2+a^2)^2} = \frac{2s}{(s^2+a^2)^2} = \underline{\underline{\frac{s}{s^2+a^2}}}$$

$$\textcircled{6} \quad L(\sinh at) = \int_0^{\infty} e^{-st} \sinh at \, dt$$

$$\sinh at = \frac{e^{at} - e^{-at}}{2}$$

$$\cosh at = \frac{e^{at} + e^{-at}}{2}$$

$$L(\sinh at) = L\left(\frac{e^{at} - e^{-at}}{2}\right) = \frac{L(e^{at}) - L(e^{-at})}{2}$$

$$= \frac{\frac{1}{s-a} - \frac{1}{s+a}}{2} = \frac{s+a - (s-a)}{(s^2-a^2)^2}$$

$$= \underline{\underline{\frac{a}{s^2-a^2}}}$$

$$\textcircled{7} \quad L(\cosh at) = L\left(\frac{e^{at} + e^{-at}}{2}\right)$$

$$= \frac{L(e^{at}) + L(e^{-at})}{2} = \frac{\frac{1}{s-a} + \frac{1}{s+a}}{2}$$

$$= \frac{s+a + s-a}{(s^2-a^2)^2} = \underline{\underline{\frac{s}{s^2-a^2}}}$$

Linear Property

If a, b, c be any constants and f, g, h any functions
t, then $L[af(t) + bg(t)] = aL(f(t)) + bL(g(t))$

First shifting Property

If $L(f(t)) = \bar{f}(s)$, then

$$L(e^{at} f(t)) = \bar{f}(s-a)$$

By ① $L(e^{at}) = \frac{1}{s-a}$

② $L(e^{at} e^{bt}) = \frac{1}{(s-b)-a}$

③ $L(e^{at} t^n) = \frac{n!}{(s-a)^{n+1}}$

④ $L(e^{at} \sin bt) = \frac{b}{(s-a)^2 + b^2}$

⑤ $L(e^{at} \cos bt) = \frac{s-a}{(s-a)^2 + b^2}$

⑥ $L(e^{at} \sinh at) = \frac{s-a}{(s-a)^2 - b^2}$

⑦ $L(e^{at} \sinh at) = \frac{a \cdot b}{(s-a)^2 - b^2}$

Transform of Periodic functions

If $f(t)$ is a periodic function with period T , i.e.

$f(t+T) = f(t)$, then

$$L(f(t)) = \frac{\int_0^T e^{-st} f(t) dt}{1 - e^{-sT}}$$

Transform of derivatives

If $f'(t)$ is continuous and $L(f(t)) = \bar{f}(s)$, then $L(f'(t)) = s\bar{f}(s) - f(0)$

$$L(f^n(t)) = s^n \bar{f}(s) - s^{n-1} f(0) - s^{n-2} f'(0) - \dots - f^{(n-1)}(0)$$

Transform of Integrals

If $L(f(t)) = \bar{f}(s)$, then $L\left\{\int_0^t f(u) du\right\} = \frac{1}{s} \bar{f}(s)$

Multiplication by t^n

If $L(f(t)) = \bar{f}(s)$, then

$$L(t^n f(t)) = (-1)^n \frac{d^n}{ds^n} (\bar{f}(s)), \quad \text{where } n=1, 2, 3, \dots$$

Convolution theorem

$$\text{If } L^{-1}\{f(s)\} = f(t) \text{ and } L^{-1}\{g(s)\} = g(t)$$

$$L^{-1}\{f(s)g(s)\} = \int_0^t f(u)g(t-u)du = F * G$$

$F * G$ is the convolution of F and G .

Inverse Laplace Transforms

$$\textcircled{1} L^{-1}\left(\frac{1}{s}\right) = 1$$

$$\textcircled{2} L^{-1}\left(\frac{1}{s-a}\right) = e^{at}$$

$$\textcircled{3} L^{-1}\left(\frac{1}{s^n}\right) = \frac{t^{n-1}}{(n-1)!}, \quad n=1, 2, 3, \dots$$

$$\textcircled{4} L^{-1}\left(\frac{1}{(s-a)^n}\right) = \frac{e^{at} t^{n-1}}{(n-1)!}$$

$$\textcircled{5} L^{-1}\left(\frac{1}{s^2+a^2}\right) = \frac{1}{a} \sin at$$

$$\textcircled{6} L^{-1}\left(\frac{s}{s^2+a^2}\right) = \cos at$$

$$\textcircled{7} L^{-1}\left(\frac{1}{s^2-a^2}\right) = \frac{1}{a} \sinh at$$

$$(8) L^{-1} \left(\frac{s}{s^2 - a^2} \right) = \cosh at$$

$$(9) L^{-1} \left(\frac{1}{(s-a)^2 + b^2} \right) = \frac{1}{b} \sin bt e^{at}$$

$$(10) L^{-1} \left(\frac{s-a}{(s-a)^2 + b^2} \right) = e^{at} \cos bt$$

$$(11) L^{-1} \left(\frac{s}{(s^2 + a^2)^2} \right) = \frac{1}{2a} t \sin at$$

$$(12) L^{-1} \left(\frac{1}{(s^2 + a^2)^2} \right) = \frac{1}{2a^3} (\sin at - at \cos at)$$

Proof: $L(t \sin at) = \frac{2as}{(s^2 + a^2)^2}$

$$L(t \cos at) = \frac{s^2 - a^2}{(s^2 + a^2)^2}$$

$$t \sin at = 2a L^{-1} \left(\frac{s}{(s^2 + a^2)^2} \right)$$

$$t \cos at = L^{-1} \left(\frac{s^2 - a^2}{(s^2 + a^2)^2} \right) = L^{-1} \left(\frac{(s^2 + a^2) - 2a^2}{(s^2 + a^2)^2} \right)$$

$$t \cos at = L^{-1} \left(\frac{1}{(s^2 + a^2)^2} \right) - 2a^2 L^{-1} \left(\frac{1}{(s^2 + a^2)^2} \right)$$

$$t \cos at = \frac{1}{a} \sin at - 2a^2 L^{-1} \left(\frac{1}{(s^2 + a^2)^2} \right)$$

$$\Rightarrow L^{-1} \left(\frac{1}{(s^2 + a^2)^2} \right) = \frac{1}{2a^3} (\sin at - at \cos at) //$$